theories/Pre_orders/Must/Alternative_Preorder/Co_Inductive/Equivalence/SoundnessCI.v
@@ -34,56 +34,10 @@ Require Import Coq.Program.Equality.
 From Coq.Logic Require Import ProofIrrelevance.
 From stdpp Require Import base countable finite gmap list finite base decidable finite gmap.
 From Must Require Import ActTau InputOutputActions gLts Bisimulation Lts_OBA Lts_OBA_FB Lts_FW FiniteImageLTS
-            Subset_Act Must Soundness Completeness Equivalence StateTransitionSystems
+            Subset_Act Must SoundnessAS CompletenessAS EquivalenceAS StateTransitionSystems
               GeneralizeLtsOutputs Termination WeakTransitions Convergence  
                InteractionBetweenLts MultisetLTSConstruction ForwarderConstruction ParallelLTSConstruction
-               Testing_Predicate.
-
-CoInductive copre `{@FiniteImagegLts A L HL LtsP, @FiniteImagegLts B L HL LtsQ}
-  `{PreAP : @PreExtAction L HL A FinA PreA PreA_eq PreA_countable 𝝳 Φ LtsP}
-  `{PreAQ : @PreExtAction L HL B FinA PreA PreA_eq PreA_countable 𝝳 Φ LtsQ}
-  (ps : gset A) (q : B) : Prop := {
-    c_tau q' : q ⟶ q' -> copre ps q'
-  ; c_now : (forall p, p ∈ ps -> p ⤓) -> q ↛ ->
-            exists p p', p ∈ ps /\ p ⟹ p' /\ p' ↛ /\ pre_co_actions_of p' ⊆ pre_co_actions_of q
-  ; c_step : forall μ q' ps', (forall p, p ∈ ps -> p ⇓ [μ]) ->
-                         q ⟶[μ] q' -> wt_set_from_pset_spec ps [μ] ps' -> copre ps' q'
-  ; c_cnv : (forall p, p ∈ ps -> p ⤓) -> q ⤓
-  }.
-
-Notation "p ⩽ q" := (copre p q) (at level 70).
-
-Lemma copre_if_prex
-  `{@FiniteImagegLts A L HL LtsP, @FiniteImagegLts B L HL LtsQ}
-  `{PreAP : @PreExtAction L HL A FinA PreA PreA_eq PreA_countable 𝝳 Φ LtsP}
-  `{PreAQ : @PreExtAction L HL B FinA PreA PreA_eq PreA_countable 𝝳 Φ LtsQ}
-  (ps : gset A) (q : B) : ps ≼ₓ q -> ps ⩽ q.
-Proof.
-  revert ps q.
-  cofix H2.
-  intros ps q (hsub1 & hsub2).
-  constructor.
-  - intros q' l. eapply H2, bhvx_preserved_by_tau; eauto.
-  - intros hterm hst.
-    edestruct (hsub2 [] q) as (p' & hw & p'' & hstp' & stable & hsub0).
-    eapply wt_nil. eassumption. intros p' mem. constructor.
-    eapply hterm. eauto.
-    exists p'. exists p''. repeat split; eauto.
-  - intros μ q' ps' hcnv hw wtspec.
-    eapply H2.
-    eapply bhvx_preserved_by_mu; eauto.
-    intros p0 mem0.
-    edestruct (hcnv p0 mem0); eauto.
-  - intros. edestruct (hsub1 []); eauto.
-    intros. constructor. eauto.
-Qed.
-
-Lemma co_preserved_by_wt_nil
-  `{@FiniteImagegLts A L HL LtsP, @FiniteImagegLts B L HL LtsQ}
-  `{PreAP : @PreExtAction L HL A FinA PreA PreA_eq PreA_countable 𝝳 Φ LtsP}
-  `{PreAQ : @PreExtAction L HL B FinA PreA PreA_eq PreA_countable 𝝳 Φ LtsQ}
-  (ps : gset A) (q q' : B) : q ⟹ q' -> ps ⩽ q -> ps ⩽ q'.
-Proof. intro hw. dependent induction hw; eauto. destruct 1. eauto. Qed.
+               Testing_Predicate DefinitionAS DefinitionCI.
 
 Lemma prex1_if_copre
   `{@FiniteImagegLts A L HL LtsP, @FiniteImagegLts B L HL LtsQ}
@@ -95,9 +49,9 @@ Proof.
   intros s hcnv.
   revert ps q H1 hcnv.
   dependent induction s; intros ps q H1 hcnv; destruct H1.
-  + constructor. eapply c_cnv0.
+  + constructor. eapply c_cnv.
     intros. now destruct (hcnv p H1).
-  +  assert (q ⤓) by (now eapply c_cnv0; intros; destruct (hcnv p H1)).
+  +  assert (q ⤓) by (now eapply c_cnv; intros; destruct (hcnv p H1)).
      assert (hcnv0 : ∀ p : A, p ∈ ps → p ⇓ [a]).
      intros p' mem'%hcnv.
      constructor. now destruct mem'.
@@ -111,7 +65,7 @@ Proof.
      eapply IHs; eauto.
      ++ eapply co_preserved_by_wt_nil. eassumption.
         eapply (co_preserved_by_wt_nil ps q q0') in hpre. destruct hpre.
-        eapply (c_step1 a q1'); eauto.
+        eapply (c_step0 a q1'); eauto.
         eapply (wt_s_set_from_pset_ispec ps [a] hcnv0); eauto. eassumption.
      ++ intros p mem.
         edestruct (wt_s_set_from_pset_ispec ps [a] hcnv0).
@@ -132,10 +86,10 @@ Proof.
   + intros q' hw hstq' hcnv.
     dependent induction hw; try rename p into q.
     ++ destruct hsub.
-       edestruct c_now0.
+       edestruct c_now.
        intros p0 mem0. edestruct (hcnv p0 mem0); eauto. eassumption.
        decompose record H1. repeat eexists;  eauto.
-    ++ eapply IHhw; eauto. destruct hsub. eapply c_tau0. eassumption.
+    ++ eapply IHhw; eauto. destruct hsub. eapply c_tau. eassumption.
   + intros. rename a into μ.
     replace (μ :: s) with ([μ] ++ s) in H1 by eauto.
     eapply wt_split in H1 as (q0 & hw0 & hw1).
@@ -148,7 +102,7 @@ Proof.
     set (ps' := wt_s_set_from_pset ps [μ] hcnv').
     assert (ps ⩽ q0') by (eapply co_preserved_by_wt_nil; eauto).
     assert (ps' ⩽ q1'). destruct H1.
-    eapply c_step0. eassumption. eassumption.
+    eapply c_step. eassumption. eassumption.
     eapply wt_s_set_from_pset_ispec.
     assert (ps' ⩽ q0) by (eapply co_preserved_by_wt_nil; eauto).
     edestruct (IHs ps' q0 H6 _ hw1 H2) 
@@ -165,51 +119,3 @@ Proof.
 Qed.
 
 
-Theorem eqx `{@FiniteImagegLts A L HL LtsP, @FiniteImagegLts B L HL LtsQ} 
-  `{PreAP : @PreExtAction L HL A FinA PreA PreA_eq PreA_countable 𝝳 Φ LtsP}
-  `{PreAQ : @PreExtAction L HL B FinA PreA PreA_eq PreA_countable 𝝳 Φ LtsQ}
-  (X : gset A) (q : B) :
-  X ≼ₓ q <-> X ⩽ q.
-Proof.
-  split.
-  - eapply copre_if_prex.
-  - intros hco. split. now eapply prex1_if_copre. now eapply prex2_if_copre.
-Qed.
-
-Section eq_contextual.
-  
-  Context `{H : ExtAction A}.
-  Context `{gLtsP : !gLts P A, !FiniteImagegLts P A}.
-  Context `{gLtsQ : !gLts Q A, !FiniteImagegLts Q A}.
-  Context `{gLtsE : !gLts E A, !FiniteImagegLts E A}.
-
-  Context `{@gLtsObaFB P A H gLtsP gLtsEqP gLtsObaP}.
-  Context `{@gLtsObaFB Q A H gLtsQ gLtsEqQ gLtsObaQ}.
-  Context `{@gLtsObaFB E A H gLtsE gLtsEqE gLtsObaE}.
-
-  Context `{attaboy : E -> Prop}.
-  Context `{attaboy_dec : forall e, Decision (attaboy e)}.
-  Context `{!Testing_Predicate E A attaboy}.
-
-  (* ************************************************** *)
-  Context `{@Prop_of_Inter P E A parallel_inter H gLtsP gLtsE}.
-  Context `{@Prop_of_Inter Q E A parallel_inter H gLtsQ gLtsE}.
-  Context `{@Prop_of_Inter P (mb A) A fw_inter H gLtsP MbgLts}.
-  Context `{@Prop_of_Inter (P * mb A) E A parallel_inter H (inter_lts fw_inter) gLtsE}.
-  Context `{@Prop_of_Inter Q (mb A) A fw_inter H gLtsQ MbgLts}.
-  Context `{@Prop_of_Inter (Q * mb A) E A parallel_inter H (inter_lts fw_inter) gLtsE}.
-
-  Context `{@PreExtAction A H (P * mb A) FinA PreA PreA_eq PreA_countable 𝝳 Φ (FW_gLts gLtsP)}.
-  Context `{@PreExtAction A H (Q * mb A) FinA PreA PreA_eq PreA_countable 𝝳 Φ (FW_gLts gLtsQ)}.
-  Context `{@AbsAction A H E FinA gLtsE Φ}.
-
-  Context `{igen_conv : @gen_spec_conv E _ _ _ _ attaboy Testing_Predicate0 co_of gen_conv}.
-  Context `{igen_acc : @gen_spec_acc PreA _ _ E _ _ _ _ attaboy Testing_Predicate0 co_of gen_acc (fun x => 𝝳 (Φ x))}.
-
-  Theorem eq_ctx (p : P) (q : Q) :
-    @pre_extensional P Q _ _ _ attaboy _ p q <-> {[ p ▷ (∅ : mb A) ]} ⩽ q ▷ (∅ : mb A).
-  Proof.
-    rewrite <- eqx, <- alt_set_singleton_iff.
-    now rewrite equivalence_bhv_acc_ctx.
-  Qed.
-End eq_contextual.
