theories/Pre_orders/Must/Must.v
@@ -345,60 +345,7 @@ Proof.
   contradiction.
 Qed.
 
-(********************************************* Alt-preorder of Must_i **********************************************)
-
-
-Definition bhv_pre_cond1 `{gLts P A, gLts Q A} 
-  (p : P) (q : Q) := forall s, p ⇓ s -> q ⇓ s.
-
-Notation "p ≼₁ q" := (bhv_pre_cond1 p q) (at level 70).
-
-(* Class of preactions.
-  Each state can only reduce for finitely many preactions *)
-
-
-(********************************** Infinite Branching Lts to Finite Branching Lts **********************)
-Class AbsAction `{H : ExtAction A} {E FinA : Type} (LtsE : @gLts E A H) (Φ : A → FinA) :=
-  MkAbsAction {
-    abstraction_test_spec μ μ' e : blocking μ -> blocking μ' -> (Φ μ) = (Φ μ') -> ¬ e ↛[ μ ] -> ¬ e ↛[ μ' ]
-  }.
-
-
-(********************************** PreCoAct modulo Finite Branching Lts on Test **********************)
-Class PreExtAction `{H : ExtAction A} {P FinA: Type} `{Countable PreAct} 
-  {𝝳 : FinA → PreAct} {Φ : A → FinA} (LtsP : @gLts P A H) :=
-  MkPreExtAction {
-      pre_co_actions_of_fin : P -> FinA -> Prop ;
-
-      preactions_of_fin_test_spec1 (μ : A) (p : P) : μ ∈ co_actions_of p -> (Φ μ) ∈ (pre_co_actions_of_fin p);
-      preactions_of_fin_test_spec2 (pre_μ : FinA) (p : P) : pre_μ ∈ (pre_co_actions_of_fin p) 
-            -> ∃ μ', μ' ∈ co_actions_of p /\ pre_μ = (Φ μ');
-
-      pre_co_actions_of : P -> gset PreAct;
-      preactions_of_spec1 (pre_μ : FinA) (p : P) : pre_μ ∈ (pre_co_actions_of_fin p) 
-        -> (𝝳 pre_μ) ∈ (pre_co_actions_of p);
-      preactions_of_spec2 (pre_pre_μ : PreAct) (pre_μ : FinA) (p : P) : 
-      (𝝳 pre_μ) = pre_pre_μ -> pre_pre_μ ∈ (pre_co_actions_of p) 
-        -> pre_μ ∈ (pre_co_actions_of_fin p);
-  }.
-
-Definition bhv_pre_cond2 `{
-  LtsP : @gLts P A H, PreAP : @PreExtAction A H P FinA PreA PreA_eq PreA_countable 𝝳 Φ LtsP,
-  LtsQ : @gLts Q A H, PreAQ : @PreExtAction A H Q FinA PreA PreA_eq PreA_countable 𝝳 Φ LtsQ}
-  (p : P) (q : Q) :=
-  forall s q',
-    p ⇓ s -> q ⟹[s] q' -> q' ↛ ->
-    ∃ p', p ⟹[s] p' /\ p' ↛ /\ (pre_co_actions_of p' ⊆ pre_co_actions_of q').
-
-Notation "p ≼₂ q" := (bhv_pre_cond2 p q) (at level 70).
-
-Definition bhv_pre `{PreA_countable : Countable PreA} `{
-  LtsP : @gLts P A H, PreAP : @PreExtAction A _ P FiniteA PreA _ _ 𝝳 Φ LtsP,
-  LtsQ : @gLts Q A H, PreAQ : @PreExtAction A _ Q FiniteA PreA _ _ 𝝳 Φ LtsQ}
-    (p : P) (q : Q) := 
-      p ≼₁ q /\ p ≼₂ q.
-
-Notation "p ≼ q" := (bhv_pre p q) (at level 70).
+From Must Require Import DefinitionAS.
 
 (** Must sets. *)
 
@@ -446,6 +393,11 @@ Section failure.
   Definition fail_pre_ms_cond2 `{@FiniteImagegLts P A H gLtsP, @FiniteImagegLts Q A H gLtsQ} 
     (p : P) (q : Q) :=
     forall s G, Failure q s G -> Failure p s G.
+
+  Definition bhv_pre_cond1 `{gLts P A, gLts Q A} 
+  (p : P) (q : Q) := forall s, p ⇓ s -> q ⇓ s.
+
+  Notation "p ≼₁ q" := (bhv_pre_cond1 p q) (at level 70).
 
   Definition fail_pre_ms `{@FiniteImagegLts P A H gLtsP, @FiniteImagegLts Q A H gLtsQ} 
     (p : P) (q : Q) :=
