theories/Labelled_Transition_System/Exemples_of_LTS/VCCS/VCCS_Instance.v
@@ -2249,6 +2249,8 @@ Proof.
   simpl. intros. inversion H. eauto.
 Qed.
 
+From Must Require Import DefinitionAS.
+
 #[global] Program Instance gAbsAction {A : Type} 
   : @AbsAction (ExtAct TypeOfActions) gLabel_b proc FinA VCCS_ggLts Φ.
 Next Obligation.
