theories/Pre_orders/Must/Alternative_Preorder/Acceptance_Set/DefinitionAS.v
@@ -1,0 +1,83 @@
+(*
+   Copyright (c) 2024 Nomadic Labs
+   Copyright (c) 2024 Paul Laforgue <paul.laforgue@nomadic-labs.com>
+   Copyright (c) 2024 Léo Stefanesco <leo.stefanesco@mpi-sws.org>
+   Copyright (c) 2025 Gaëtan Lopez <glopez@irif.fr>
+
+   Permission is hereby granted, free of charge, to any person obtaining a copy
+   of this software and associated documentation files (the "Software"), to deal
+   in the Software without restriction, including without limitation the rights
+   to use, copy, modify, merge, publish, distribute, sublicense, and/or sell
+   copies of the Software, and to permit persons to whom the Software is
+   furnished to do so, subject to the following conditions:
+
+   The above copyright notice and this permission notice shall be included in all
+   copies or substantial portions of the Software.
+
+   THE SOFTWARE IS PROVIDED "AS IS", WITHOUT WARRANTY OF ANY KIND, EXPRESS OR
+   IMPLIED, INCLUDING BUT NOT LIMITED TO THE WARRANTIES OF MERCHANTABILITY,
+   FITNESS FOR A PARTICULAR PURPOSE AND NONINFRINGEMENT. IN NO EVENT SHALL THE
+   AUTHORS OR COPYRIGHT HOLDERS BE LIABLE FOR ANY CLAIM, DAMAGES OR OTHER
+   LIABILITY, WHETHER IN AN ACTION OF CONTRACT, TORT OR OTHERWISE, ARISING FROM,
+   OUT OF OR IN CONNECTION WITH THE SOFTWARE OR THE USE OR OTHER DEALINGS IN THE
+   SOFTWARE.
+*)
+
+From Coq.Unicode Require Import Utf8.
+From Coq.Program Require Import Equality.
+From stdpp Require Import finite gmap decidable.
+From Must Require Import ActTau gLts Bisimulation Lts_OBA Subset_Act WeakTransitions Testing_Predicate
+    StateTransitionSystems InteractionBetweenLts Convergence Termination FiniteImageLTS.
+
+(********************************************* Alt-preorder of Must_i **********************************************)
+
+
+(********************************** Infinite Branching Lts to Finite Branching Lts **********************)
+Class AbsAction `{H : ExtAction A} {E FinA : Type} (LtsE : @gLts E A H) (Φ : A → FinA) :=
+  MkAbsAction {
+    abstraction_test_spec μ μ' e : blocking μ -> blocking μ' -> (Φ μ) = (Φ μ') -> ¬ e ↛[ μ ] -> ¬ e ↛[ μ' ]
+  }.
+
+
+(********************************** PreCoAct modulo Finite Branching Lts on Test **********************)
+Class PreExtAction `{H : ExtAction A} {P FinA: Type} `{Countable PreAct} 
+  {𝝳 : FinA → PreAct} {Φ : A → FinA} (LtsP : @gLts P A H) :=
+  MkPreExtAction {
+      pre_co_actions_of_fin : P -> FinA -> Prop ;
+
+      preactions_of_fin_test_spec1 (μ : A) (p : P) : μ ∈ co_actions_of p -> (Φ μ) ∈ (pre_co_actions_of_fin p);
+      preactions_of_fin_test_spec2 (pre_μ : FinA) (p : P) : pre_μ ∈ (pre_co_actions_of_fin p) 
+            -> ∃ μ', μ' ∈ co_actions_of p /\ pre_μ = (Φ μ');
+
+      pre_co_actions_of : P -> gset PreAct;
+      preactions_of_spec1 (pre_μ : FinA) (p : P) : pre_μ ∈ (pre_co_actions_of_fin p) 
+        -> (𝝳 pre_μ) ∈ (pre_co_actions_of p);
+      preactions_of_spec2 (pre_pre_μ : PreAct) (pre_μ : FinA) (p : P) : 
+      (𝝳 pre_μ) = pre_pre_μ -> pre_pre_μ ∈ (pre_co_actions_of p) 
+        -> pre_μ ∈ (pre_co_actions_of_fin p);
+  }.
+
+
+Definition bhv_pre_cond1 `{gLts P A, gLts Q A} 
+  (p : P) (q : Q) := forall s, p ⇓ s -> q ⇓ s.
+
+Notation "p ≼₁ q" := (bhv_pre_cond1 p q) (at level 70).
+
+Definition bhv_pre_cond2 `{
+  LtsP : @gLts P A H, PreAP : @PreExtAction A H P FinA PreA PreA_eq PreA_countable 𝝳 Φ LtsP,
+  LtsQ : @gLts Q A H, PreAQ : @PreExtAction A H Q FinA PreA PreA_eq PreA_countable 𝝳 Φ LtsQ}
+  (p : P) (q : Q) :=
+  forall s q',
+    p ⇓ s -> q ⟹[s] q' -> q' ↛ ->
+    ∃ p', p ⟹[s] p' /\ p' ↛ /\ (pre_co_actions_of p' ⊆ pre_co_actions_of q').
+
+Notation "p ≼₂ q" := (bhv_pre_cond2 p q) (at level 70).
+
+Definition bhv_pre `{PreA_countable : Countable PreA} `{
+  LtsP : @gLts P A H, PreAP : @PreExtAction A _ P FiniteA PreA _ _ 𝝳 Φ LtsP,
+  LtsQ : @gLts Q A H, PreAQ : @PreExtAction A _ Q FiniteA PreA _ _ 𝝳 Φ LtsQ}
+    (p : P) (q : Q) := 
+      p ≼₁ q /\ p ≼₂ q.
+
+Notation "p ≼ q" := (bhv_pre p q) (at level 70).
+
