theories/Pre_orders/Must/Alternative_Preorder/Co_Inductive/DefinitionCI.v
@@ -1,0 +1,63 @@
+(*
+   Copyright (c) 2024 Nomadic Labs
+   Copyright (c) 2024 Paul Laforgue <paul.laforgue@nomadic-labs.com>
+   Copyright (c) 2024 Léo Stefanesco <leo.stefanesco@mpi-sws.org>
+
+   Permission is hereby granted, free of charge, to any person obtaining a copy
+   of this software and associated documentation files (the "Software"), to deal
+   in the Software without restriction, including without limitation the rights
+   to use, copy, modify, merge, publish, distribute, sublicense, and/or sell
+   copies of the Software, and to permit persons to whom the Software is
+   furnished to do so, subject to the following conditions:
+
+   The above copyright notice and this permission notice shall be included in all
+   copies or substantial portions of the Software.
+
+   THE SOFTWARE IS PROVIDED "AS IS", WITHOUT WARRANTY OF ANY KIND, EXPRESS OR
+   IMPLIED, INCLUDING BUT NOT LIMITED TO THE WARRANTIES OF MERCHANTABILITY,
+   FITNESS FOR A PARTICULAR PURPOSE AND NONINFRINGEMENT. IN NO EVENT SHALL THE
+   AUTHORS OR COPYRIGHT HOLDERS BE LIABLE FOR ANY CLAIM, DAMAGES OR OTHER
+   LIABILITY, WHETHER IN AN ACTION OF CONTRACT, TORT OR OTHERWISE, ARISING FROM,
+   OUT OF OR IN CONNECTION WITH THE SOFTWARE OR THE USE OR OTHER DEALINGS IN THE
+   SOFTWARE.
+*)
+
+Require ssreflect.
+Require Import Coq.Unicode.Utf8.
+Require Import Coq.Lists.List.
+Import ListNotations.
+Require Import Coq.Program.Equality.
+Require Import Coq.Wellfounded.Inverse_Image.
+Require Import Coq.Logic.JMeq.
+Require Import Coq.Program.Wf Setoid.
+Require Import Coq.Program.Equality.
+From Coq.Logic Require Import ProofIrrelevance.
+From stdpp Require Import base countable finite gmap list finite base decidable finite gmap.
+From Must Require Import ActTau InputOutputActions gLts Bisimulation Lts_OBA Lts_OBA_FB Lts_FW FiniteImageLTS
+            Subset_Act Must SoundnessAS CompletenessAS EquivalenceAS StateTransitionSystems
+              GeneralizeLtsOutputs Termination WeakTransitions Convergence  
+               InteractionBetweenLts MultisetLTSConstruction ForwarderConstruction ParallelLTSConstruction
+               Testing_Predicate DefinitionAS.
+
+CoInductive copre `{@FiniteImagegLts A L HL LtsP, @FiniteImagegLts B L HL LtsQ}
+  `{PreAP : @PreExtAction L HL A FinA PreA PreA_eq PreA_countable 𝝳 Φ LtsP}
+  `{PreAQ : @PreExtAction L HL B FinA PreA PreA_eq PreA_countable 𝝳 Φ LtsQ}
+  (ps : gset A) (q : B) : Prop := {
+    c_tau q' : q ⟶ q' -> copre ps q'
+  ; c_now : (forall p, p ∈ ps -> p ⤓) -> q ↛ ->
+            exists p p', p ∈ ps /\ p ⟹ p' /\ p' ↛ /\ pre_co_actions_of p' ⊆ pre_co_actions_of q
+  ; c_step : forall μ q' ps', (forall p, p ∈ ps -> p ⇓ [μ]) ->
+                         q ⟶[μ] q' -> wt_set_from_pset_spec ps [μ] ps' -> copre ps' q'
+  ; c_cnv : (forall p, p ∈ ps -> p ⤓) -> q ⤓
+  }.
+
+Notation "p ⩽ q" := (copre p q) (at level 70).
+
+Lemma co_preserved_by_wt_nil
+  `{@FiniteImagegLts A L HL LtsP, @FiniteImagegLts B L HL LtsQ}
+  `{PreAP : @PreExtAction L HL A FinA PreA PreA_eq PreA_countable 𝝳 Φ LtsP}
+  `{PreAQ : @PreExtAction L HL B FinA PreA PreA_eq PreA_countable 𝝳 Φ LtsQ}
+  (ps : gset A) (q q' : B) : q ⟹ q' -> ps ⩽ q -> ps ⩽ q'.
+Proof. intro hw. dependent induction hw; eauto. destruct 1. eauto. Qed.
+
+
